Add BT of fvar and bvar

src/Bohm_Tree.lean
@@ -49,14 +49,17 @@ lemma normal_or_redex (T : Term Var) : isHeadRedex T ∨ isHeadNormal T := by
       · cases ih1 ; left ; apply isHeadRedex.base ; apply isHeadRedexApp.step ; assumption
       · cases ih1 ; right ; apply isHeadNormal.base ; apply isHeadNormalApp.step ; assumption
 
+@[simp]
 def nfoldAbs : ℕ → Term Var → Term Var
 | 0, T => T
 | n + 1, T => nfoldAbs n T.abs
 
+@[simp]
 def nfoldOpen : List Var → Term Var → Term Var
 | [], T => T
 | a :: as, T => nfoldOpen as (T.open' (Term.fvar a))
 
+@[simp]
 def nfoldApp : List (Term Var) → Term Var → Term Var
 | [], T => T
 | a :: as, T => nfoldApp as (T.app a)
@@ -165,6 +168,51 @@ theorem hnf_mono (t : bfvar Var) : monotone fun f ↦ BöhmTree.hnf 1 0 t fun _ 
   right
   constructor <;> try rfl
   grind [coherent, CoInd.leN_le, monotone]
+
+-- BT of free variable together with correctness proof
+def BT_fvar (n : Var) : BöhmTree Var := .hnf 0 0 ⟨Term.fvar n, by simp⟩ (fun n ↦ .no_hnf)
+lemma BT_fvar_correct (n : Var) : BT Var (Term.fvar n) [] (BT_fvar n) := by
+  unfold BT_fvar
+  apply BT.hnf_free_fvar Var _ [] n []
+  · simp [hasAsHnf]
+    constructor
+    · apply isHeadNormal.base
+      apply isHeadNormalApp.base_free
+    · apply Relation.EqvGen.refl
+  · simp only [List.length_nil, List.get_eq_getElem, IsEmpty.exists_iff, not_false_eq_true]
+  . simp only [List.length_nil, List.append_nil, Fin.getElem_fin, IsEmpty.forall_iff]
+
+
+-- BT of bound variable together with correctness proof
+def BT_bvar (n : ℕ) : BöhmTree Var := .hnf 0 0 ⟨Term.bvar n, by simp⟩ (fun n ↦ .no_hnf)
+lemma BT_bvar_correct (n : ℕ) : BT Var (Term.bvar n) [] (BT_bvar n) := by
+  unfold BT_bvar
+  apply BT.hnf_bvar Var _ [] n []
+  · simp [hasAsHnf]
+    constructor
+    · apply isHeadNormal.base
+      apply isHeadNormalApp.base_bound
+    · apply Relation.EqvGen.refl
+  · simp only [List.length_nil, List.append_nil, Fin.getElem_fin, nfoldOpen, IsEmpty.forall_iff]
+
+-- Var : Type u
+-- P Q : Term Var
+-- ihP : ∃ L T, BT Var P L T
+-- ihQ : ∃ L T, BT Var Q L T
+-- ⊢ ∃ L T, BT Var (P.app Q) L T
+-- def BT_app (P Q : Term Var) : BöhmTree Var := sorry
+
+lemma exists_BT_for_term (M : Term Var) : ∃ L T, BT Var M L T := by
+  induction M with
+  | bvar n =>
+    exact ⟨[], BT_bvar n, BT_bvar_correct _⟩
+  | fvar x => exact ⟨[], BT_fvar x, BT_fvar_correct _⟩
+  | app P Q ihP ihQ =>
+    obtain ⟨LP, TP⟩ := ihP
+    obtain ⟨LQ, TQ⟩ := ihQ
+    sorry
+  | abs => sorry
+
 
 def inf_Ytree : BöhmTree Var :=
   .hnf 1 0 ⟨Term.bvar 0, by simp⟩ (λ _ ↦ inf_Ytree)
